WIP: Implement LinkedList internals with selectors

examples/steel/Steel.Sel.LList.fsti
@@ -36,7 +36,7 @@ let llist (#a:Type0) (r:t a) = VUnit (llist' r)
 
 [@@ __steel_reduce__]
 let v_llist (#a:Type0) (#p:vprop) (r:t a)
-  (h:rmem p{FStar.Tactics.with_tactic selector_tactic (can_be_split p (llist r) /\ True)})
+  (h:rmem p{FStar.Tactics.with_tactic selector_tactic (can_be_split p (llist r) /\ True)}) : GTot (list a)
   = h (llist r)
 
 val intro_llist_nil (a:Type0)
@@ -49,6 +49,12 @@ val intro_llist_cons (#a:Type0) (ptr1 ptr2:t a)
                   (fun _ -> llist ptr1)
                   (requires fun h -> next (sel ptr1 h) == ptr2)
                   (ensures fun h0 _ h1 -> v_llist ptr1 h1 == (data (sel ptr1 h0)) :: v_llist ptr2 h0)
+
+val reveal_non_empty (#a:Type0) (ptr:t a)
+  : SteelSel unit (llist ptr) (fun _ -> llist ptr)
+             (requires fun _ -> ptr =!= null_llist)
+             (ensures fun h0 _ h1 -> v_llist ptr h0 == v_llist ptr h1 /\ Cons? (v_llist ptr h0))
+
 
 val tail (#a:Type0) (ptr:t a)
   : SteelSel (t a) (llist ptr)
